feat: `Nat` inequalities in cutsat (#7494)
This PR implements support for `Nat` inequalities in the cutsat
procedure.

src/Init/Data/Int/OfNat.lean
@@ -26,6 +26,7 @@ inductive Expr where
   | mul  (a b : Expr)
   | div  (a b : Expr)
   | mod  (a b : Expr)
+  deriving BEq
 
 def Expr.denote (ctx : Context) : Expr → Nat
   | .num k    => k
@@ -57,5 +58,13 @@ theorem Expr.le (ctx : Context) (lhs rhs : Expr)
 theorem Expr.dvd (ctx : Context) (lhs rhs : Expr)
     : (lhs.denote ctx ∣ rhs.denote ctx) = (lhs.denoteAsInt ctx ∣ rhs.denoteAsInt ctx) := by
   simp [denoteAsInt_eq, Int.ofNat_dvd]
+
+theorem of_nat_le (ctx : Context) (lhs rhs : Expr)
+    : lhs.denote ctx ≤ rhs.denote ctx → lhs.denoteAsInt ctx ≤ rhs.denoteAsInt ctx := by
+  rw [Expr.le ctx lhs rhs]; simp
+
+theorem of_not_nat_le (ctx : Context) (lhs rhs : Expr)
+    : ¬ lhs.denote ctx ≤ rhs.denote ctx → ¬ lhs.denoteAsInt ctx ≤ rhs.denoteAsInt ctx := by
+  rw [Expr.le ctx lhs rhs]; simp
 
 end Int.OfNat
