src/Lean/Meta/Tactic/Grind/Arith/Cutsat/Nat.lean
@@ -74,17 +74,13 @@ partial def toOfNatExpr (e : Lean.Expr) : M Expr := do
 
 /--
 Given `e` of the form `lhs ≤ rhs` where `lhs` and `rhs` have type `Nat`,
-returns `(lhs', rhs', h)` where `lhs'` and `rhs'` are integer expressions and `h` is a proof
-that `(lhs ≤ rhs) = (lhs', rhs')`
+returns `(lhs, rhs, ctx)` where `lhs` and `rhs` are `Int.OfNat.Expr` and `ctx` is the context.
 -/
-def toIntLe? (e : Lean.Expr) : MetaM (Option (Lean.Expr × Lean.Expr × Lean.Expr)) := do
+def toIntLe? (e : Lean.Expr) : MetaM (Option (Expr × Expr × Array Lean.Expr)) := do
   let_expr LE.le _ inst lhs rhs := e | return none
   unless (← isInstLENat inst) do return none
   let ((lhs, rhs), s) ← conv lhs rhs |>.run {}
-  let lhs' := lhs.denoteAsIntExpr s.ctx
-  let rhs' := rhs.denoteAsIntExpr s.ctx
-  let h := mkApp3 (mkConst ``Int.OfNat.Expr.le) (Simp.Arith.Nat.toContextExpr s.ctx) (toExpr lhs) (toExpr rhs)
-  return some (lhs', rhs', h)
+  return some (lhs, rhs, s.ctx)
 where
   conv (lhs rhs : Lean.Expr) : M (Expr × Expr) :=
     return (← toOfNatExpr lhs, ← toOfNatExpr rhs)
