tests/lean/run/grind_cutsat_nat_le.lean
@@ -1,0 +1,17 @@
+set_option grind.warning false
+
+theorem ex1 (x y z : Nat) : x < y + z → y + 1 < z → z + x < 3*z := by
+  grind
+
+theorem ex2 {p : Prop} (x y z : Nat) : x < y + z → y + 1 < z → (p ↔ z + x < 3*z) → p := by
+  grind
+
+theorem ex3 (x y : Nat) :
+    27 ≤ 13*x + 11*y → 13*x + 11*y ≤ 30 →
+    7*y ≤ 9*x + 10 → 9*x ≤ 4 + 7*y → False := by
+  grind
+
+open Int.Linear Int.OfNat
+#print ex1
+#print ex2
+#print ex3
